theories/check_fo.v
@@ -1,6 +1,6 @@
 From det Require Import prelude.
 From mathcomp Require Import all_ssreflect.
-From det Require Import tree tree_prop ctx tree_vars unif mut_excl.
+From det Require Import tree tree_prop ctx tree_vars unif mut_excl fresh.
 
 Section checker.
 
